compiler/backend/proofs/clos_numberProofScript.sml
@@ -874,10 +874,7 @@ val renumber_code_locs_correct = Q.store_thm("renumber_code_locs_correct",
     Cases_on `r1` \\ full_simp_tac(srw_ss())[] >> srw_tac[][] >> full_simp_tac(srw_ss())[] >>
     full_simp_tac(srw_ss())[find_code_def] >>
     `FDOM s2'.code = FDOM t2.code` by full_simp_tac(srw_ss())[state_rel_def,fmap_rel_def] >>
-    BasicProvers.CASE_TAC >> full_simp_tac(srw_ss())[] >- (
-      full_simp_tac(srw_ss())[FLOOKUP_DEF] >>
-      srw_tac[][] ) >>
-    rfs[state_rel_def])
+    fs [FLOOKUP_DEF,state_rel_def])
   THEN1 (* App empty *)
    (full_simp_tac(srw_ss())[evaluate_def] >> srw_tac[][])
   THEN1 (* Real App *)
@@ -978,7 +975,7 @@ val renumber_code_locs_elist_globals = Q.store_thm(
       set_globals e' = set_globals e)`,
   ho_match_mp_tac renumber_code_locs_ind >>
   simp[renumber_code_locs_def] >> rpt strip_tac >>
-  rpt (pairarg_tac >> fs[]) >> rveq >> fs[] >>
+  rpt (pairarg_tac >> fs[]) >> rveq >> fs[EVAL ``op_gbag Add``] >>
   rename1`renumber_code_locs_list locn1 (MAP SND functions)` >>
   qspecl_then [`locn1`, `MAP SND functions`] mp_tac
     (CONJUNCT1 renumber_code_locs_length) >>
